Modified examples for weak/strong causality. Added one example. Moved and renamed examples for better overview.

TStreamCaseStudy_DS.thy
@@ -15,25 +15,65 @@ begin
 lemma tstake1of1tick: "Abs_tstream (\<up>\<surd>) \<down> 1 = Abs_tstream (\<up>\<surd>)"
 by (simp add: tsTake_def2 One_nat_def)
 
-lemma tstake1of2tick: "Abs_tstream (<[\<surd>, \<surd>]>) \<down> 1 = Abs_tstream (\<up>\<surd>)"
-by (simp add: tsTake_def2 One_nat_def tstakefirst_insert_rep_eq)
-
 lemma tstake2of1tick: "Abs_tstream (\<up>\<surd>) \<down> 2 = Abs_tstream (\<up>\<surd>)"
 using tstake1of1tick tstake_fin2 by fastforce
+
+lemma tstake1of2tick: "Abs_tstream (<[\<surd>, \<surd>]>) \<down> 1 = Abs_tstream (\<up>\<surd>)"
+by (simp add: tsTake_def2 One_nat_def tstakefirst_insert_rep_eq)
 
 lemma tstake2of2tick: "Abs_tstream (<[\<surd>, \<surd>]>) \<down> 2 = Abs_tstream (<[\<surd>, \<surd>]>)"
 by (smt One_nat_def Rep_Abs list2s.simps(2) list2s_0 lscons_conv numeral_2_eq_2 sup'_def tick_msg
     tsconc_insert tstake1of1tick tstake_tick)
 
-lemma tstake2ofinftick: "(tsinftimes (Abs_tstream (\<up>\<surd>))) \<down> 2 = Abs_tstream (<[\<surd>, \<surd>]>)"
-by (smt One_nat_def Rep_Abs Rep_cfun_strict1 Suc_1 list2s.simps(2) list2s_0 lscons_conv sup'_def 
-    tick_msg tsDropTake1 tsTake.simps(1) tsTakeDrop tsconc_assoc tsconc_insert tsinftimes_unfold
-    tstake2of2tick tstake_tick)
+lemma tstake1ofinftick: "(tsinftimes (Abs_tstream (\<up>\<surd>))) \<down> 1 = Abs_tstream (\<up>\<surd>)"
+by (metis One_nat_def Rep_cfun_strict1 tsDropTake1 tsTake.simps(1) tsTakeDrop tsinftimes_unfold
+    tstake2of1tick tstake_tick)
 
-lemma tstakenofinftick: "#(Rep_tstream tsinftimes (Abs_tstream (\<up>\<surd>)) \<down> n) < \<infinity>"
+lemma tstake2ofinftick: "(tsinftimes (Abs_tstream (\<up>\<surd>))) \<down> 2 = Abs_tstream (<[\<surd>, \<surd>]>)"
+by (metis Rep_Abs Suc_1 list2s.simps(2) list2s_0 lscons_conv sconc_snd_empty tick_msg tsconc_insert
+    tsinftimes_unfold tstake1ofinftick tstake_tick)
+
+lemma slen_tstakenofinftick: "#(Rep_tstream tsinftimes (Abs_tstream (\<up>\<surd>)) \<down> n) < \<infinity>"
 by (metis Abs_Rep Inf'_neq_0 Rep_tstream_strict inf_ub less_le sconc_fst_inf sconc_snd_empty
     slen_empty_eq tsDropNth tsDropTake1 ts_well_Rep ts_well_def tsconc_insert tsinf_nth
     tstake_tsnth tstickcount_insert)
+
+lemma slen_inftick: "#(Rep_tstream (tsinftimes (Abs_tstream (\<up>\<surd>)))) = \<infinity>"
+by (metis (no_types, lifting) less_irrefl ln_less sConc_Rep_fin_fin slen_scons tick_msg tsInfTicks
+    tsconc_rep_eq tsinftimes_unfold tstickcount_insert)
+
+lemma not_below_2tick_tick: "Abs_tstream (\<up>\<surd> \<bullet> \<up>\<surd>) \<notsqsubseteq> Abs_tstream (\<up>\<surd>)"
+by (smt Rep_Abs Rep_tstream_inject list2s.simps(1) list2s.simps(2) list2s_inj lscons_conv 
+    not_Cons_self po_eq_conv sup'_def tick_msg ts_tsconc_prefix ts_well_conc1 tsconc_rep_eq1)
+
+
+
+(* Constructed non monotone function on tstreams is not continous but weak causal *)
+definition tsnonmono :: "'a tstream \<Rightarrow> 'a tstream" where
+"tsnonmono ts \<equiv> if ts=\<bottom> then Abs_tstream (\<up>\<surd>) else \<bottom>"
+
+(* \<bottom> \<sqsubseteq> x but <\<surd>> \<sqsubseteq> \<bottom> is false *)
+lemma non_mono_tsnonmono: "\<not>monofun tsnonmono"
+by (simp add: monofun_def tsnonmono_def)
+
+lemma non_cont_tsnonmono: "\<not>cont tsnonmono"
+using cont2mono non_mono_tsnonmono by auto
+
+lemma tsweak_tsnonmono: "tsWeakCausal tsnonmono"
+apply (rule tsWeakCausalI)
+apply (simp add: tsnonmono_def, auto)
+using tstakeBot by blast+
+
+(* Constructed non monotone function on tstreams is not strong causal
+   \<bottom> \<down> 0 = <\<surd>> \<down> 0 but \<bottom> \<down> 1 \<noteq> <\<surd>> \<down> 1 *)
+lemma non_tsstrong_tsnonmono: "\<not>tsStrongCausal tsnonmono"
+apply(auto simp add: tsnonmono_def tsStrongCausal_def)
+apply (rule_tac x=0 in exI)
+apply (rule_tac x="Abs_tstream (\<up>\<surd>)" in exI)
+by (metis One_nat_def Rep_Abs Rep_cfun_strict1 Rep_tstream_bottom_iff stream.con_rews(2) sup'_def
+    tick_msg tsTake.simps(1) tstake1of1tick up_defined)
+
+
 
 (* Constructed non continous function on tstreams is monotone and weak causal *)
 definition tsmonoweak :: "'a tstream \<Rightarrow> 'a tstream" where
@@ -54,7 +94,7 @@ by (metis ln_less neq_iff slen_scons tick_msg tsconc_rep_eq tsinftimes_unfold)
 
 lemma tsmonoweak_inftick_is_ub:
   "range (\<lambda>i. tsmonoweak tsinftimes (Abs_tstream (\<up>\<surd>)) \<down> i ) <| tsinftimes (Abs_tstream (\<up>\<surd>))"
-by (simp add: is_ub_def tsmonoweak_def tstakenofinftick)
+by (simp add: is_ub_def tsmonoweak_def slen_tstakenofinftick)
 
 lemma non_cont_tsmonoweak: "\<not>cont tsmonoweak"
 apply (simp add: cont_def)
